\begin{verbatim}
f($x) = exp($x) - 3*$x**2
f'($x) = exp($x) - 6*$x
Initial guess = secant 0
Initial guess 2 = 0.5
  0, 0.5
  0.5, 4.93687078675298
  4.93687078675298, 0.438951196275084
  0.438951196275084, 0.371867885050184
  0.371867885050184, 1.48270060759859
  1.48270060759859, 0.728462521279268
  0.728462521279268, 0.864018097840986
  0.864018097840986, 0.916037072232311
  0.916037072232311, 0.909838202019623
  0.909838202019623, 0.910006972136034
  0.910006972136034, 0.910007572548784
  0.910007572548784, 0.910007572488709
0.910007572488709
\end{verbatim}
