\documentclass[12pt]{article}

\usepackage[black-square,define-standard-theorems,dont-number-theorems]{QED}
\usepackage{amsmath}
\usepackage{amssymb}

\begin{document}
\noindent Luke Palmer \\
2005-02-07 \\
MATH 4230

\begin{description}
\item[(1.5.13)]
\begin{gather*}
\beta(s) = \left( \int_0^s{\cos{\theta(u)}\,du},
                  \int_0^s{\sin{\theta(u)}\,du} \right) \\
T(s) = \beta'(s) = (\cos{\theta(s)}, \sin{\theta(s)}) \\
|\beta'(s)| = 1 
\intertext{So $\beta$ is unit speed.}
T'(s) = \kappa(s) N(s) = (-\theta'(s) \sin{\theta(s)}, \theta'(s) \cos{\theta(s)}) \\
|T'(s)| = |\kappa(s) N(s)| = |\kappa(s)| = |\theta'(s)|  \\
\theta(s) \equiv \int_0^s{\kappa(s)\,ds}\text{, so } \theta'(s) = \kappa(s).
\end{gather*}

\item[(1.5.15)]
\begin{gather*}
\theta(s) = \int_0^s{\kappa(u)\,du} = \int_0^s{\frac{du}{1+u^2}} = \tan^{-1}(s) \\
\beta'(s) = (\cos{\tan^{-1}(s)}, \sin{\tan^{-1}(s)}) \\
\beta(s) = (\sinh^{-1}(s), \sqrt{s^2+1}-1)
\end{gather*}

\item[(1.5.17)]

\begin{Theorem}
Given unit-speed parameterizations of curves $\alpha(s)$ and
$\beta(s)$, with $\kappa_\alpha(s) = \kappa_\beta(s)$ and
$\tau_\alpha(s) = \tau_\beta(s)$, $\alpha$ is equivalent to $\beta$
under some rigid motion (translation and rotation).
\end{Theorem}

\begin{Proof}
Define a unitary matrix $\mathbf{R}$ so that the Frenet frames
$\mathbf{F}_\alpha(0) = \mathbf{R} \mathbf{F}_\beta(0)$.  Let $\beta^* =
\mathbf{R}\beta$.

Consider the function:

\begin{align*}
D(s) &= T_\alpha(s) \cdot T_{\beta^*}(s) +
        N_\alpha(s) \cdot N_{\beta^*}(s) +
        B_\alpha(s) \cdot B_{\beta^*}(s) \\
     &= T_\alpha(s) \cdot \mathbf{R}T_\beta(s) +
        N_\alpha(s) \cdot \mathbf{R}N_\beta(s) +
        B_\alpha(s) \cdot \mathbf{R}B_\beta(s)
\end{align*}

Since $T$, $N$, and $B$ of both curves are unit-speed, and $\mathbf{R}$
is unitary, $D(s) \le 3$ for every $s$ due to the triangle inequality.
Also, $D(s_0) = 3$ only when $\mathbf{F}_\alpha = \mathbf{F}_{\beta^*}$.
We've defined this to be true at $s = 0$, so $D(0) = 3$.

Consider:

\begin{align*}
D'(s) = &T'_\alpha \cdot \mathbf{R}T_{\beta} + T_\alpha \cdot \mathbf{R}T'_{\beta} \\
      + &N'_\alpha \cdot \mathbf{R}N_{\beta} + N_\alpha \cdot \mathbf{R}N'_{\beta} \\
      + &B'_\alpha \cdot \mathbf{R}B_{\beta} + B_\alpha \cdot \mathbf{R}B'_{\beta} \\
      = &\kappa N_\alpha \cdot \mathbf{R}T_{\beta} + T_\alpha \cdot \kappa \mathbf{R} N_\beta \\
      + &(-\kappa T_\alpha + \tau B_\alpha) \cdot \mathbf{R} N_\beta + 
            N_\alpha \cdot \mathbf{R} (-\kappa T_\beta +\tau B_\beta) \\
      + &-\tau N_\alpha \cdot \mathbf{R} B_\beta - \tau B_\alpha \cdot \mathbf{R} N_\beta
\intertext{...After expanding and eliminating common terms with opposite
signs...}
      = &0
\end{align*}

$D(s)$ never changes from 3, so the frenet frames correspond at all
points.  For unit-speed curves, $T$ defines the derivative of the curve,
so $\alpha$ and $\beta^*$ are equivalent under translation.

\end{Proof}

\end{description}
\end{document}
